back to lax with bounds

proofs/fstar/extraction-edited/Libcrux.Kem.Kyber.Arithmetic.fst
@@ -3,23 +3,60 @@ module Libcrux.Kem.Kyber.Arithmetic
 open Core
 open FStar.Mul
 
+
+let lemma_mul_i32_range (n1 n2:i32) (b1 b2:nat):
+  Lemma (requires (i32_range n1 b1 /\ i32_range n2 b2 /\ b1 * b2 < pow2 31))
+        (ensures (range (v n1 * v n2) i32_inttype /\
+                  i32_range (n1 *! n2) (b1 * b2)))
+  = if v n1 = 0 || v n2 = 0 then ()
+    else 
+    let open FStar.Math.Lemmas in
+    lemma_abs_bound (v n1) b1;
+    lemma_abs_bound (v n2) b2;
+    lemma_abs_mul (v n1) (v n2);
+    lemma_mult_le_left (abs (v n1)) (abs (v n2)) b2;
+    lemma_mult_le_right b2 (abs (v n1)) b1;
+    lemma_abs_bound (v n1 * v n2) (b1 * b2)
+
+
+let lemma_add_i32_range (n1 n2:i32) (b1 b2:nat):
+  Lemma (requires (i32_range n1 b1 /\ i32_range n2 b2 /\ b1 + b2 < pow2 31))
+        (ensures (range (v n1 + v n2) i32_inttype /\
+                  i32_range (n1 +! n2) (b1 + b2)))
+  = ()
+
+let mul_i32_b #b1 #b2 x y = 
+  lemma_mul_i32_range x y b1 b2;
+  x *! y
+
+let add_i32_b #b1 #b2 x y = 
+  lemma_add_i32_range x y b1 b2;
+  x +! y
+
+let sub_i32_b #b1 #b2 x y = 
+  x -! y
+
+let cast_i32_b #b1 #b2 x =
+  x <: i32_b b2
+
 let v_MONTGOMERY_R: i32 = 1l <<! v_MONTGOMERY_SHIFT
 
 let mont_to_spec_fe (m:t_FieldElement) = admit()
 
-#push-options "--fuel 0 --ifuel 1 --z3rlimit 100"
+#push-options "--fuel 0 --ifuel 1 --z3rlimit 200"
 let get_n_least_significant_bits n value = 
   let _:Prims.unit = () <: Prims.unit in
   let res = value &. ((1ul <<! n <: u32) -! 1ul <: u32) in
   logand_mask_lemma value (v n);
-  assert (bounded res (v n));
+  assert (v res <= v n);
   res
 #pop-options 
 
-let barrett_reduce (value: i32) = 
+let barrett_reduce value = 
   let _:Prims.unit = () <: Prims.unit in
+  let x : i32 = value in
   let t:i64 =
-    ((Core.Convert.f_from value <: i64) *! v_BARRETT_MULTIPLIER <: i64) +!
+    ((Core.Convert.f_from x <: i64) *! v_BARRETT_MULTIPLIER <: i64) +!
     (v_BARRETT_R >>! 1l <: i64)
   in
   let quotient:i32 = cast (t >>! v_BARRETT_SHIFT <: i64) <: i32 in
@@ -28,7 +65,7 @@ let barrett_reduce (value: i32) =
   admit();
   result
 
-let montgomery_reduce (value: i32) = 
+let montgomery_reduce value = 
   let _:i32 = v_MONTGOMERY_R in
   let _:Prims.unit = () <: Prims.unit in
   let t:u32 =
@@ -45,12 +82,12 @@ let montgomery_reduce (value: i32) =
   admit(); // P-F
   res
 
-let montgomery_multiply_sfe_by_fer (fe fer: i32) =
-  montgomery_reduce (fe *! fer <: i32)
+let montgomery_multiply_sfe_by_fer fe fer =
+  montgomery_reduce (mul_i32_b fe fer)
 
 
-let to_standard_domain (mfe: i32) =
-  montgomery_reduce (mfe *! v_MONTGOMERY_R_SQUARED_MOD_FIELD_MODULUS <: i32)
+let to_standard_domain mfe =
+  montgomery_reduce (mul_i32_b mfe (v_MONTGOMERY_R_SQUARED_MOD_FIELD_MODULUS <: i32_b 1353))
 
 let to_unsigned_representative (fe: i32) =
   let _:Prims.unit = () <: Prims.unit in
@@ -63,25 +100,51 @@ let to_unsigned_representative (fe: i32) =
   admit(); //P-F
   res
 
-let add_to_ring_element (v_K: usize) (lhs rhs: t_PolynomialRingElement) = 
+let derefine_poly_b #b x =
+  let r = createi (sz 256) (fun i -> (x.f_coefficients.[i] <: i32)) in
+  {f_coefficients = r}
+
+let derefine_vector_b #p #b x =
+  let r = createi (p.v_RANK) (fun i -> derefine_poly_b #b x.[i]) in
+  r
+
+let derefine_matrix_b #p #b x =
+  let r = createi (p.v_RANK) (fun i -> derefine_vector_b #p #b x.[i]) in
+  r
+
+let cast_poly_b #b1 #b2 x =
+  let r = createi (sz 256) (fun i -> (x.f_coefficients.[i] <: i32_b b2)) in
+  let res = {f_coefficients = r} in
+  let dx = (derefine_poly_b x).f_coefficients in
+  let dr = (derefine_poly_b res).f_coefficients in
+  assert (forall (i:usize). v i < 256 ==> 
+    (dx.[i] <: i32) == 
+    (dr.[i] <: i32));
+  assert (forall i. Seq.index dx i == (dx.[sz i] <: i32));
+  eq_intro dx dr;
+  assert(Seq.equal dx dr);
+  res
+
+let add_to_ring_element #b1 #b2 v_K lhs rhs =
   let _:Prims.unit = () <: Prims.unit in
   let _:Prims.unit = () <: Prims.unit in
   let orig_lhs = lhs in
   [@ inline_let]
-  let inv = fun (acc:t_PolynomialRingElement) (i:usize) ->
+  let inv = fun (acc:t_PolynomialRingElement_b (b1+b2)) (i:usize) ->
       (forall j. j <. i ==> acc.f_coefficients.[j] == lhs.f_coefficients.[j] +! rhs.f_coefficients.[j]) /\
       (forall j. j >=. i ==> acc.f_coefficients.[j] == orig_lhs.f_coefficients.[j]) in
-  let lhs:t_PolynomialRingElement =
-    Rust_primitives.Iterators.foldi_range #_ #(t_PolynomialRingElement)  #inv {
+  let lhs:t_PolynomialRingElement_b (b1 + b2) =
+    Rust_primitives.Iterators.foldi_range #_ #(t_PolynomialRingElement_b (b1+b2))  #inv {
               Core.Ops.Range.f_start = sz 0;
               Core.Ops.Range.f_end =
-              Core.Slice.impl__len (Rust_primitives.unsize lhs.f_coefficients <: t_Slice i32)
+              Core.Slice.impl__len (Rust_primitives.unsize lhs.f_coefficients <: t_Slice (i32_b b1))
             }
-      lhs
+      (cast_poly_b #b1 #(b1+b2) lhs)
       (fun lhs i ->
-          let lhs:t_PolynomialRingElement = lhs in
+          let lhs:t_PolynomialRingElement_b (b1+b2) = lhs in
           let i:usize = i in
           assert (orig_lhs.f_coefficients.[i] == lhs.f_coefficients.[i]);
+          let lhsi: i32_b b1 = orig_lhs.f_coefficients.[i] in
           let lhs = 
           {
             lhs with
@@ -89,12 +152,12 @@ let add_to_ring_element (v_K: usize) (lhs rhs: t_PolynomialRingElement) =
             =
             Rust_primitives.Hax.Monomorphized_update_at.update_at_usize lhs.f_coefficients
               i
-              ((lhs.f_coefficients.[ i ] <: i32) +! (rhs.f_coefficients.[ i ] <: i32) <: i32)
+              (add_i32_b #b1 #b2 (lhsi) (rhs.f_coefficients.[ i ]))
             <:
-            t_Array i32 (sz 256)
+            t_Array (i32_b (b1 + b2)) (sz 256)
           }
           <:
-          t_PolynomialRingElement
+          t_PolynomialRingElement_b (b1 + b2)
           in
           assert (forall j. (j >. i /\ j <. sz 256) ==> lhs.f_coefficients.[j] == orig_lhs.f_coefficients.[j]);
           lhs
@@ -102,6 +165,7 @@ let add_to_ring_element (v_K: usize) (lhs rhs: t_PolynomialRingElement) =
   in
   let _:Prims.unit = () <: Prims.unit in
   assert (forall j. j <. sz 256 ==> lhs.f_coefficients.[j] == orig_lhs.f_coefficients.[j] +! rhs.f_coefficients.[j]);
-  lhs 
+  lhs
   
   
+ 
