proofs/fstar/extraction-edited/Libcrux.Kem.Kyber.Arithmetic.fsti
@@ -3,8 +3,24 @@ module Libcrux.Kem.Kyber.Arithmetic
 open Core
 open FStar.Mul
 
+let i32_range (n:i32) (b:nat) =
+  b < pow2 31 /\ v n <= b /\ v n >= -b
+
+type i32_b b = x:i32{i32_range x b}
+
+val mul_i32_b (#b1:nat) (#b2:nat{b1 * b2 < pow2 31}) (x:i32_b b1) (y: i32_b b2): r:i32_b (b1 * b2){v r == v x * v y}
+val add_i32_b (#b1:nat) (#b2:nat{b1 + b2 < pow2 31}) (x:i32_b b1) (y: i32_b b2): r:i32_b (b1 + b2){v r == v x + v y}
+val sub_i32_b (#b1:nat) (#b2:nat{b1 + b2 < pow2 31}) (x:i32_b b1) (y: i32_b b2): r:i32_b (b1 + b2){v r == v x - v y}
+val cast_i32_b (#b1:nat) (#b2:nat{b1 <= b2 /\ b2 < pow2 31}) (x:i32_b b1): r:i32_b b2{v r == v x}
+
 unfold
 let t_FieldElement = i32
+
+unfold
+let t_FieldElement_b b = i32_b b
+
+unfold
+let wfFieldElement = t_FieldElement_b 3328
 
 unfold
 let t_FieldElementTimesMontgomeryR = i32
@@ -26,12 +42,15 @@ let v_MONTGOMERY_SHIFT: u8 = 16uy
 
 val v_MONTGOMERY_R: x:i32{v x = pow2 16}
 
-let to_spec_fe (m:t_FieldElement) : Spec.Kyber.field_element = 
+let to_spec_fe (m:i32) : Spec.Kyber.field_element = 
     let m_v = v m % v Libcrux.Kem.Kyber.Constants.v_FIELD_MODULUS in
     assert (m_v > -  v Libcrux.Kem.Kyber.Constants.v_FIELD_MODULUS);
     if m_v < 0 then
       m_v + v Libcrux.Kem.Kyber.Constants.v_FIELD_MODULUS
     else m_v
+
+let to_spec_fe_b #b (m:i32_b b) : Spec.Kyber.field_element = to_spec_fe m
+
 
 val mont_to_spec_fe (m:t_FieldElement)
     : Spec.Kyber.field_element
@@ -45,30 +64,34 @@ val get_n_least_significant_bits (n: u8 {v n > 0 /\ v n <= 32}) (value: u32)
           v result = v value % pow2 (v n))
 
 
-let barrett_pre (value:i32) = 
-    v value <= v v_BARRETT_R /\ v value >= - v v_BARRETT_R
+//let barrett_pre (value:i32) = 
+//    v value <= v v_BARRETT_R /\ v value >= - v v_BARRETT_R
 // Appears to work up to +/- 2^28, but not at +/- 2^29
 
 let barrett_post (value:i32) (result:i32) = 
     v result % v Libcrux.Kem.Kyber.Constants.v_FIELD_MODULUS =
-    v value % v Libcrux.Kem.Kyber.Constants.v_FIELD_MODULUS /\
-    v result > - (v Libcrux.Kem.Kyber.Constants.v_FIELD_MODULUS) /\
-    v result < (v Libcrux.Kem.Kyber.Constants.v_FIELD_MODULUS)
+    v value % v Libcrux.Kem.Kyber.Constants.v_FIELD_MODULUS
+//    /\
+//    v result > - (v Libcrux.Kem.Kyber.Constants.v_FIELD_MODULUS) /\
+//    v result < (v Libcrux.Kem.Kyber.Constants.v_FIELD_MODULUS)
 
-val barrett_reduce (value: i32)
-    : Prims.Pure i32
-    (requires barrett_pre value)
-    (ensures barrett_post value)
+val barrett_reduce (value: i32_b (v v_BARRETT_R))
+    : Prims.Pure wfFieldElement
+    (requires True)
+    (ensures fun r -> barrett_post value r)
 
 let montgomery_post (value:i32) (result:i32) =
     v result % v Libcrux.Kem.Kyber.Constants.v_FIELD_MODULUS =
-    (v value / v v_MONTGOMERY_R) % v Libcrux.Kem.Kyber.Constants.v_FIELD_MODULUS /\
+    (v value / v v_MONTGOMERY_R) % v Libcrux.Kem.Kyber.Constants.v_FIELD_MODULUS
+    
+(*    /\
    (let abs_v = abs (v value) in
     v result >= - (abs_v / v v_MONTGOMERY_R) - v Libcrux.Kem.Kyber.Constants.v_FIELD_MODULUS / 2 /\
     v result <= (abs_v / v v_MONTGOMERY_R) + v Libcrux.Kem.Kyber.Constants.v_FIELD_MODULUS / 2)
+*)
 
-val montgomery_reduce (value: i32)
-    : Prims.Pure i32
+val montgomery_reduce #b (value: i32_b b)
+    : Prims.Pure (i32_b ((b / v v_MONTGOMERY_R) + v Libcrux.Kem.Kyber.Constants.v_FIELD_MODULUS/2))
       (requires True)
       (ensures
         fun result ->
@@ -76,33 +99,62 @@ val montgomery_reduce (value: i32)
           montgomery_post value result)
 
 
-val montgomery_multiply_sfe_by_fer (fe fer: i32) 
+val montgomery_multiply_sfe_by_fer #b1 #b2 (fe:i32_b b1) (fer: i32_b b2)
     : Pure i32
-      (requires (range (v fe * v fer) i32_inttype))
+      (requires (b1 * b2 < pow2 31))
       (ensures (fun result -> 
-          montgomery_post (fe *! fer) (result)))
+          montgomery_post (mul_i32_b fe fer) (result)))
       
 
-val to_standard_domain (mfe: i32) 
+val to_standard_domain #b (mfe: i32_b b) 
     : Pure i32
-      (requires (range (v mfe * 1353) i32_inttype))
+      (requires (b * 1353 < pow2 31))
       (ensures (fun result -> 
-          montgomery_post (mfe *! 1353l) result))
+          montgomery_post (mul_i32_b mfe (1353l <: i32_b 1353)) result))
 
-let to_unsigned_representative_pre (fe: i32)
-  = fe >=. (Core.Ops.Arith.Neg.neg Libcrux.Kem.Kyber.Constants.v_FIELD_MODULUS <: i32) &&
-    fe <. Libcrux.Kem.Kyber.Constants.v_FIELD_MODULUS
 
-val to_unsigned_representative (fe: i32)
+val to_unsigned_representative (fe: wfFieldElement)
     : Prims.Pure (int_t_d u16_inttype 12)
-      (requires to_unsigned_representative_pre fe)
+      (requires True)
       (ensures
         fun result ->
           let result:u16 = result in
+          v result == to_spec_fe fe /\
           result >=. 0us &&
           result <. (cast (Libcrux.Kem.Kyber.Constants.v_FIELD_MODULUS <: i32) <: u16))
 
-type t_PolynomialRingElement = { f_coefficients:t_Array i32 (sz 256) }
+type t_PolynomialRingElement = { f_coefficients:t_Array (t_FieldElement) (sz 256) }
+
+type t_PolynomialRingElement_b b = { f_coefficients:t_Array (i32_b b) (sz 256) }
+
+type wfPolynomialRingElement = t_PolynomialRingElement_b (v Libcrux.Kem.Kyber.Constants.v_FIELD_MODULUS)
+
+val derefine_poly_b (#b1:nat) (x:t_PolynomialRingElement_b b1):  
+    r:t_PolynomialRingElement{
+    forall (i:usize). v i < 256 ==> (r.f_coefficients.[i] <: i32) ==  (x.f_coefficients.[i] <: i32)}
+
+val derefine_vector_b (#p:Spec.Kyber.params) (#b:nat) (x:t_Array (t_PolynomialRingElement_b b) p.v_RANK):
+    r:t_Array t_PolynomialRingElement p.v_RANK{
+    forall (i j:usize). (v i < v p.v_RANK /\ v j < 256) ==>
+     (let ri : t_PolynomialRingElement = r.[i] in
+      let xi : t_PolynomialRingElement_b b = x.[i] in
+      (ri.f_coefficients.[j] <: i32) == 
+      (xi.f_coefficients.[j] <: i32))}
+
+val derefine_matrix_b (#p:Spec.Kyber.params) (#b:nat) 
+  (x:t_Array (t_Array (t_PolynomialRingElement_b b) p.v_RANK) p.v_RANK) :
+    r:t_Array (t_Array t_PolynomialRingElement p.v_RANK) p.v_RANK{
+    forall (i j k:usize). (v i < v p.v_RANK /\ v j < v p.v_RANK /\ v k < 256) ==>
+     (let ri : t_Array (t_PolynomialRingElement) p.v_RANK = r.[i] in
+      let xi : t_Array (t_PolynomialRingElement_b b) p.v_RANK = x.[i] in
+      let rij : t_PolynomialRingElement = ri.[j] in
+      let xij : t_PolynomialRingElement_b b = xi.[j] in
+      (rij.f_coefficients.[k] <: i32) == 
+      (xij.f_coefficients.[k] <: i32))}
+
+val cast_poly_b (#b1:nat) (#b2:nat{b1 <= b2 /\ b2 < pow2 31}) 
+  (x:t_PolynomialRingElement_b b1): r:t_PolynomialRingElement_b b2{
+    derefine_poly_b x == derefine_poly_b r}
 
 let op_String_Access #t #l (a:t_Array t l) (i:usize{v i < v l}) : t = a.[i]
 
@@ -112,38 +164,58 @@ let to_spec_poly (m:t_PolynomialRingElement) : (Spec.Kyber.polynomial) =
     assert (forall i. Seq.index p i < v Spec.Kyber.v_FIELD_MODULUS);
     p
 
+let to_spec_poly_b #b (m:t_PolynomialRingElement_b b) : (Spec.Kyber.polynomial) =
+    to_spec_poly (derefine_poly_b m)
+
 let mont_to_spec_poly (m:t_PolynomialRingElement) : (Spec.Kyber.polynomial) =
     let p = createi #nat (sz 256) (fun i -> mont_to_spec_fe (m.f_coefficients.[i])) in
     assert (forall i. Seq.index p i = mont_to_spec_fe (m.f_coefficients.[sz i]));
     assert (forall i. Seq.index p i < v Spec.Kyber.v_FIELD_MODULUS);
     p
 
+
 let to_spec_vector (#p:Spec.Kyber.params)
-                   (m:t_Array t_PolynomialRingElement p.v_RANK)
+                   (m:t_Array (t_PolynomialRingElement) p.v_RANK)
                    : (Spec.Kyber.vector p) =
     createi p.v_RANK (fun i -> to_spec_poly (m.[i]))
 
+
+let to_spec_vector_b (#p:Spec.Kyber.params) (#b:nat)
+                   (m:t_Array (t_PolynomialRingElement_b b) p.v_RANK)
+                   : (Spec.Kyber.vector p) =
+    to_spec_vector (derefine_vector_b m)
+
 let mont_to_spec_vector (#p:Spec.Kyber.params)
-                   (m:t_Array t_PolynomialRingElement p.v_RANK)
+                   (m:t_Array (t_PolynomialRingElement) p.v_RANK)
                    : (Spec.Kyber.vector p) =
     createi p.v_RANK (fun i -> mont_to_spec_poly (m.[i]))
 
-let to_spec_matrix (#p:Spec.Kyber.params)
-                   (m:(t_Array (t_Array t_PolynomialRingElement p.v_RANK) p.v_RANK))
+let mont_to_spec_vector_b (#p:Spec.Kyber.params) (#b:nat)
+                   (m:t_Array (t_PolynomialRingElement_b b) p.v_RANK)
+                   : (Spec.Kyber.vector p) =
+    mont_to_spec_vector (derefine_vector_b m)
+
+let to_spec_matrix (#p:Spec.Kyber.params) 
+                   (m:(t_Array (t_Array (t_PolynomialRingElement) p.v_RANK) p.v_RANK))
                    : (Spec.Kyber.matrix p) =
     createi p.v_RANK (fun i -> to_spec_vector (m.[i]))
 
-let mont_to_spec_matrix (#p:Spec.Kyber.params)
-                   (m:(t_Array (t_Array t_PolynomialRingElement p.v_RANK) p.v_RANK))
+let to_spec_matrix_b (#p:Spec.Kyber.params) (#b:nat)
+                   (m:(t_Array (t_Array (t_PolynomialRingElement_b b) p.v_RANK) p.v_RANK))
+                   : (Spec.Kyber.matrix p) =
+    to_spec_matrix (derefine_matrix_b m)
+
+let mont_to_spec_matrix (#p:Spec.Kyber.params) 
+                   (m:(t_Array (t_Array (t_PolynomialRingElement) p.v_RANK) p.v_RANK))
                    : (Spec.Kyber.matrix p) =
     createi p.v_RANK (fun i -> mont_to_spec_vector (m.[i]))
 
-let impl__PolynomialRingElement__ZERO: t_PolynomialRingElement =
-  { f_coefficients = Rust_primitives.Hax.repeat 0l (sz 256) } <: t_PolynomialRingElement
+let impl__PolynomialRingElement__ZERO: t_PolynomialRingElement_b 1 =
+  { f_coefficients = Rust_primitives.Hax.repeat (0l <: i32_b 1) (sz 256) } <: t_PolynomialRingElement_b 1
 
-val add_to_ring_element (v_K: usize) (lhs rhs: t_PolynomialRingElement)
-    : Prims.Pure t_PolynomialRingElement
-      (requires forall i. range (v lhs.f_coefficients.[i] + v rhs.f_coefficients.[i]) i32_inttype)
+val add_to_ring_element (#b1:nat) (#b2:nat{b1 + b2 < pow2 31}) (v_K: usize) (lhs: t_PolynomialRingElement_b b1) (rhs: t_PolynomialRingElement_b b2)
+    : Prims.Pure (t_PolynomialRingElement_b (b1 + b2))
+      (requires True) 
       (ensures fun result ->
         (forall i. v result.f_coefficients.[i] == v lhs.f_coefficients.[i] + v rhs.f_coefficients.[i]))
 
