proofs/fstar/extraction-edited/Libcrux.Kem.Kyber.Matrix.fst
@@ -7,56 +7,54 @@ let op_Array_Access (x:Libcrux.Kem.Kyber.Arithmetic.t_PolynomialRingElement) (i:
     x.f_coefficients.[i]
     
 
-let compute_As_plus_e
-      (v_K: usize)
-      (matrix_A: t_Array (t_Array Libcrux.Kem.Kyber.Arithmetic.t_PolynomialRingElement v_K) v_K)
-      (s_as_ntt error_as_ntt: t_Array Libcrux.Kem.Kyber.Arithmetic.t_PolynomialRingElement v_K) =
-  let result:t_Array Libcrux.Kem.Kyber.Arithmetic.t_PolynomialRingElement v_K =
+let compute_As_plus_e v_K matrix_A s_as_ntt error_as_ntt =
+  let result:t_Array Libcrux.Kem.Kyber.Arithmetic.wfPolynomialRingElement v_K =
     Rust_primitives.Hax.repeat Libcrux.Kem.Kyber.Arithmetic.impl__PolynomialRingElement__ZERO v_K
   in
-  let acc_t = t_Array Libcrux.Kem.Kyber.Arithmetic.t_PolynomialRingElement v_K in
+  admit();
+  let acc_t = t_Array Libcrux.Kem.Kyber.Arithmetic.wfPolynomialRingElement v_K in
   [@ inline_let]
   let inv = fun (acc:acc_t) (i:usize) -> True in
-  let result:t_Array Libcrux.Kem.Kyber.Arithmetic.t_PolynomialRingElement v_K =
-    Rust_primitives.Iterators.foldi_slice #(t_Array Libcrux.Kem.Kyber.Arithmetic.t_PolynomialRingElement v_K) #acc_t #inv
+  let result:t_Array Libcrux.Kem.Kyber.Arithmetic.wfPolynomialRingElement v_K =
+    Rust_primitives.Iterators.foldi_slice #(t_Array Libcrux.Kem.Kyber.Arithmetic.wfPolynomialRingElement v_K) #acc_t #inv
       matrix_A
       result
       (fun result temp_1_ ->
-          let result:t_Array Libcrux.Kem.Kyber.Arithmetic.t_PolynomialRingElement v_K = result in
-          let i, row:(usize & t_Array Libcrux.Kem.Kyber.Arithmetic.t_PolynomialRingElement v_K) =
+          let result:t_Array Libcrux.Kem.Kyber.Arithmetic.wfPolynomialRingElement v_K = result in
+          let i, row:(usize & t_Array Libcrux.Kem.Kyber.Arithmetic.wfPolynomialRingElement v_K) =
             temp_1_
           in
           [@ inline_let]
           let inv = fun (acc:acc_t) (i:usize) -> True in
-          let result:t_Array Libcrux.Kem.Kyber.Arithmetic.t_PolynomialRingElement v_K =
-            Rust_primitives.Iterators.foldi_slice #Libcrux.Kem.Kyber.Arithmetic.t_PolynomialRingElement #acc_t #inv
+          let result:t_Array Libcrux.Kem.Kyber.Arithmetic.wfPolynomialRingElement v_K =
+            Rust_primitives.Iterators.foldi_slice #Libcrux.Kem.Kyber.Arithmetic.wfPolynomialRingElement #acc_t #inv
               row
               result
               (fun result temp_1_ ->
-                  let result:t_Array Libcrux.Kem.Kyber.Arithmetic.t_PolynomialRingElement v_K =
+                  let result:t_Array Libcrux.Kem.Kyber.Arithmetic.wfPolynomialRingElement v_K =
                     result
                   in
                   let j, matrix_element:(usize &
-                    Libcrux.Kem.Kyber.Arithmetic.t_PolynomialRingElement) =
+                    Libcrux.Kem.Kyber.Arithmetic.wfPolynomialRingElement) =
                     temp_1_
                   in
-                  let product:Libcrux.Kem.Kyber.Arithmetic.t_PolynomialRingElement =
+                  let product:Libcrux.Kem.Kyber.Arithmetic.wfPolynomialRingElement =
                     Libcrux.Kem.Kyber.Ntt.ntt_multiply matrix_element
-                      (s_as_ntt.[ j ] <: Libcrux.Kem.Kyber.Arithmetic.t_PolynomialRingElement)
+                      (s_as_ntt.[ j ] <: Libcrux.Kem.Kyber.Arithmetic.wfPolynomialRingElement)
                   in
                   admit(); // needs bounds for add_to_ring_element
-                  let result:t_Array Libcrux.Kem.Kyber.Arithmetic.t_PolynomialRingElement v_K =
+                  let result:t_Array Libcrux.Kem.Kyber.Arithmetic.wfPolynomialRingElement v_K =
                     Rust_primitives.Hax.Monomorphized_update_at.update_at_usize result
                       i
                       (Libcrux.Kem.Kyber.Arithmetic.add_to_ring_element v_K
-                          (result.[ i ] <: Libcrux.Kem.Kyber.Arithmetic.t_PolynomialRingElement)
+                          (result.[ i ] <: Libcrux.Kem.Kyber.Arithmetic.wfPolynomialRingElement)
                           product
                         <:
-                        Libcrux.Kem.Kyber.Arithmetic.t_PolynomialRingElement)
+                        Libcrux.Kem.Kyber.Arithmetic.wfPolynomialRingElement)
                   in
                   result)
           in
-          let acc_t = t_Array Libcrux.Kem.Kyber.Arithmetic.t_PolynomialRingElement v_K in
+          let acc_t = t_Array Libcrux.Kem.Kyber.Arithmetic.wfPolynomialRingElement v_K in
           [@ inline_let]
           let inv = fun (acc:acc_t) (i:usize) -> True in
             Rust_primitives.Iterators.foldi_range #_ #acc_t #inv {
@@ -65,38 +63,35 @@ let compute_As_plus_e
             }
             result
             (fun result j ->
-                let result:t_Array Libcrux.Kem.Kyber.Arithmetic.t_PolynomialRingElement v_K =
+                let result:t_Array Libcrux.Kem.Kyber.Arithmetic.wfPolynomialRingElement v_K =
                   result
                 in
                 let j:usize = j in
                 assume (range (v (result.[i]).(j) * 1353) i32_inttype);
-                let coefficient_normal_form:i32 =
-                  Libcrux.Kem.Kyber.Arithmetic.to_standard_domain ((result.[ i ]
+                let coefficient_normal_form =
+                  Libcrux.Kem.Kyber.Arithmetic.to_standard_domain #3328 ((result.[ i ]
                         <:
-                        Libcrux.Kem.Kyber.Arithmetic.t_PolynomialRingElement)
-                        .Libcrux.Kem.Kyber.Arithmetic.f_coefficients.[ j ]
-                      <:
-                      i32)
+                        Libcrux.Kem.Kyber.Arithmetic.wfPolynomialRingElement)
+                        .Libcrux.Kem.Kyber.Arithmetic.f_coefficients.[ j ])
                 in
-                let x1: Libcrux.Kem.Kyber.Arithmetic.t_PolynomialRingElement = error_as_ntt.[i] in
+                let x1: Libcrux.Kem.Kyber.Arithmetic.wfPolynomialRingElement = error_as_ntt.[i] in
                 let x2 : i32 = x1.f_coefficients.[j] in
                 assume (range (v coefficient_normal_form + v x2) i32_inttype);
-                assume (Libcrux.Kem.Kyber.Arithmetic.barrett_pre (coefficient_normal_form +! x2));
                 Rust_primitives.Hax.Monomorphized_update_at.update_at_usize result
                   i
                   ({
-                      (result.[ i ] <: Libcrux.Kem.Kyber.Arithmetic.t_PolynomialRingElement) with
+                      (result.[ i ] <: Libcrux.Kem.Kyber.Arithmetic.wfPolynomialRingElement) with
                       Libcrux.Kem.Kyber.Arithmetic.f_coefficients
                       =
                       Rust_primitives.Hax.Monomorphized_update_at.update_at_usize (result.[ i ]
                           <:
-                          Libcrux.Kem.Kyber.Arithmetic.t_PolynomialRingElement)
+                          Libcrux.Kem.Kyber.Arithmetic.wfPolynomialRingElement)
                           .Libcrux.Kem.Kyber.Arithmetic.f_coefficients
                         j
                         (Libcrux.Kem.Kyber.Arithmetic.barrett_reduce (coefficient_normal_form +!
                               ((error_as_ntt.[ i ]
                                   <:
-                                  Libcrux.Kem.Kyber.Arithmetic.t_PolynomialRingElement)
+                                  Libcrux.Kem.Kyber.Arithmetic.wfPolynomialRingElement)
                                   .Libcrux.Kem.Kyber.Arithmetic.f_coefficients.[ j ]
                                 <:
                                 i32)
@@ -108,61 +103,65 @@ let compute_As_plus_e
                       t_Array i32 (sz 256)
                     }
                     <:
-                    Libcrux.Kem.Kyber.Arithmetic.t_PolynomialRingElement)))
+                    Libcrux.Kem.Kyber.Arithmetic.wfPolynomialRingElement)))
   in
   admit(); //P-F
-  result
+  result 
 
 let compute_message #p v_K m_v secret_as_ntt u_as_ntt = 
-  let result:Libcrux.Kem.Kyber.Arithmetic.t_PolynomialRingElement =
+  let result:Libcrux.Kem.Kyber.Arithmetic.wfPolynomialRingElement =
     Libcrux.Kem.Kyber.Arithmetic.impl__PolynomialRingElement__ZERO
   in
-  let acc_t = Libcrux.Kem.Kyber.Arithmetic.t_PolynomialRingElement in
+  let acc_t = Libcrux.Kem.Kyber.Arithmetic.wfPolynomialRingElement in
   [@ inline_let]
   let inv = fun (acc:acc_t) (i:usize) -> True in
-  let result:Libcrux.Kem.Kyber.Arithmetic.t_PolynomialRingElement =
+  let result:Libcrux.Kem.Kyber.Arithmetic.wfPolynomialRingElement =
     Rust_primitives.Iterators.foldi_range #_ #acc_t #inv {
               Core.Ops.Range.f_start = sz 0;
               Core.Ops.Range.f_end = v_K
             }
       result 
       (fun result i ->
-          let result:Libcrux.Kem.Kyber.Arithmetic.t_PolynomialRingElement = result in
+          let result:Libcrux.Kem.Kyber.Arithmetic.wfPolynomialRingElement = result in
           let i:usize = i in
-          let product:Libcrux.Kem.Kyber.Arithmetic.t_PolynomialRingElement =
+          admit();
+          let product:Libcrux.Kem.Kyber.Arithmetic.wfPolynomialRingElement =
             Libcrux.Kem.Kyber.Ntt.ntt_multiply (secret_as_ntt.[ i ]
                 <:
-                Libcrux.Kem.Kyber.Arithmetic.t_PolynomialRingElement)
-              (u_as_ntt.[ i ] <: Libcrux.Kem.Kyber.Arithmetic.t_PolynomialRingElement)
+                Libcrux.Kem.Kyber.Arithmetic.wfPolynomialRingElement)
+              (u_as_ntt.[ i ] <: Libcrux.Kem.Kyber.Arithmetic.wfPolynomialRingElement)
           in
           admit(); //pre for add_to_ring
-          let result:Libcrux.Kem.Kyber.Arithmetic.t_PolynomialRingElement =
+          let result:Libcrux.Kem.Kyber.Arithmetic.wfPolynomialRingElement =
             Libcrux.Kem.Kyber.Arithmetic.add_to_ring_element v_K result product
           in
           result)
   in
-  let result:Libcrux.Kem.Kyber.Arithmetic.t_PolynomialRingElement =
+  let result:Libcrux.Kem.Kyber.Arithmetic.wfPolynomialRingElement =
     Libcrux.Kem.Kyber.Ntt.invert_ntt_montgomery v_K result
   in
-  let acc_t = Libcrux.Kem.Kyber.Arithmetic.t_PolynomialRingElement in
+  let acc_t = Libcrux.Kem.Kyber.Arithmetic.wfPolynomialRingElement in
   [@ inline_let]
   let inv = fun (acc:acc_t) (i:usize) -> True in
-  let result:Libcrux.Kem.Kyber.Arithmetic.t_PolynomialRingElement =
+  let result:Libcrux.Kem.Kyber.Arithmetic.wfPolynomialRingElement =
     Rust_primitives.Iterators.foldi_range #_ #acc_t #inv {
               Core.Ops.Range.f_start = sz 0;
               Core.Ops.Range.f_end = Libcrux.Kem.Kyber.Constants.v_COEFFICIENTS_IN_RING_ELEMENT
             }
       result 
       (fun result i ->
-          let result:Libcrux.Kem.Kyber.Arithmetic.t_PolynomialRingElement = result in
+          let result:Libcrux.Kem.Kyber.Arithmetic.wfPolynomialRingElement = result in
           let i:usize = i in
-          assume (range (v result.(i) *  1441) i32_inttype);
-          let coefficient_normal_form:i32 = Libcrux.Kem.Kyber.Arithmetic.montgomery_reduce 
-                           (result.Libcrux.Kem.Kyber.Arithmetic.f_coefficients.[ i ] *! 1441l) in
-          assume (range (v m_v.(i) - v coefficient_normal_form) i32_inttype);
-          assume (Libcrux.Kem.Kyber.Arithmetic.barrett_pre (m_v.(i) -! coefficient_normal_form));
+          assume (range (v #i32_inttype result.Libcrux.Kem.Kyber.Arithmetic.f_coefficients.[i] *  1441) i32_inttype);
+          let coefficient_normal_form = 
+              Libcrux.Kem.Kyber.Arithmetic.montgomery_reduce 
+                           (Libcrux.Kem.Kyber.Arithmetic.mul_i32_b #3328 #1441
+                           result.Libcrux.Kem.Kyber.Arithmetic.f_coefficients.[ i ] 
+                           (1441l <: Libcrux.Kem.Kyber.Arithmetic.i32_b 1441)) in
+          assume (range (v #i32_inttype m_v.Libcrux.Kem.Kyber.Arithmetic.f_coefficients.[i] - v coefficient_normal_form) i32_inttype);
+//          assume (Libcrux.Kem.Kyber.Arithmetic.barrett_pre (m_v.(i) -! coefficient_normal_form));
 
-          let result:Libcrux.Kem.Kyber.Arithmetic.t_PolynomialRingElement =
+          let result:Libcrux.Kem.Kyber.Arithmetic.wfPolynomialRingElement =
             {
               result with
               Libcrux.Kem.Kyber.Arithmetic.f_coefficients
@@ -181,7 +180,7 @@ let compute_message #p v_K m_v secret_as_ntt u_as_ntt =
                   i32)
             }
             <:
-            Libcrux.Kem.Kyber.Arithmetic.t_PolynomialRingElement
+            Libcrux.Kem.Kyber.Arithmetic.wfPolynomialRingElement
           in
           result)
   in
@@ -191,12 +190,12 @@ let compute_message #p v_K m_v secret_as_ntt u_as_ntt =
 
 let compute_ring_element_v
       (v_K: usize)
-      (tt_as_ntt r_as_ntt: t_Array Libcrux.Kem.Kyber.Arithmetic.t_PolynomialRingElement v_K)
-      (error_2_ message: Libcrux.Kem.Kyber.Arithmetic.t_PolynomialRingElement) =
-  let result:Libcrux.Kem.Kyber.Arithmetic.t_PolynomialRingElement =
+      (tt_as_ntt r_as_ntt: t_Array Libcrux.Kem.Kyber.Arithmetic.wfPolynomialRingElement v_K)
+      (error_2_ message: Libcrux.Kem.Kyber.Arithmetic.wfPolynomialRingElement) =
+  let result:Libcrux.Kem.Kyber.Arithmetic.wfPolynomialRingElement =
     Libcrux.Kem.Kyber.Arithmetic.impl__PolynomialRingElement__ZERO
   in
-  let result:Libcrux.Kem.Kyber.Arithmetic.t_PolynomialRingElement =
+  let result:Libcrux.Kem.Kyber.Arithmetic.wfPolynomialRingElement =
     Core.Iter.Traits.Iterator.f_fold (Core.Iter.Traits.Collect.f_into_iter ({
               Core.Ops.Range.f_start = sz 0;
               Core.Ops.Range.f_end = v_K
@@ -207,24 +206,25 @@ let compute_ring_element_v
         Core.Ops.Range.t_Range usize)
       result
       (fun result i ->
-          let result:Libcrux.Kem.Kyber.Arithmetic.t_PolynomialRingElement = result in
+          let result:Libcrux.Kem.Kyber.Arithmetic.wfPolynomialRingElement = result in
           let i:usize = i in
-          let product:Libcrux.Kem.Kyber.Arithmetic.t_PolynomialRingElement =
+          admit();
+          let product:Libcrux.Kem.Kyber.Arithmetic.wfPolynomialRingElement =
             Libcrux.Kem.Kyber.Ntt.ntt_multiply (tt_as_ntt.[ i ]
                 <:
-                Libcrux.Kem.Kyber.Arithmetic.t_PolynomialRingElement)
-              (r_as_ntt.[ i ] <: Libcrux.Kem.Kyber.Arithmetic.t_PolynomialRingElement)
+                Libcrux.Kem.Kyber.Arithmetic.wfPolynomialRingElement)
+              (r_as_ntt.[ i ] <: Libcrux.Kem.Kyber.Arithmetic.wfPolynomialRingElement)
           in
           admit(); //pre for add_to_ring_element
-          let result:Libcrux.Kem.Kyber.Arithmetic.t_PolynomialRingElement =
+          let result:Libcrux.Kem.Kyber.Arithmetic.wfPolynomialRingElement =
             Libcrux.Kem.Kyber.Arithmetic.add_to_ring_element v_K result product
           in
           result)
   in
-  let result:Libcrux.Kem.Kyber.Arithmetic.t_PolynomialRingElement =
+  let result:Libcrux.Kem.Kyber.Arithmetic.wfPolynomialRingElement =
     Libcrux.Kem.Kyber.Ntt.invert_ntt_montgomery v_K result
   in
-  let result:Libcrux.Kem.Kyber.Arithmetic.t_PolynomialRingElement =
+  let result:Libcrux.Kem.Kyber.Arithmetic.wfPolynomialRingElement =
     Core.Iter.Traits.Iterator.f_fold (Core.Iter.Traits.Collect.f_into_iter ({
               Core.Ops.Range.f_start = sz 0;
               Core.Ops.Range.f_end = Libcrux.Kem.Kyber.Constants.v_COEFFICIENTS_IN_RING_ELEMENT
@@ -235,25 +235,22 @@ let compute_ring_element_v
         Core.Ops.Range.t_Range usize)
       result
       (fun result i ->
-          let result:Libcrux.Kem.Kyber.Arithmetic.t_PolynomialRingElement = result in
+          let result:Libcrux.Kem.Kyber.Arithmetic.wfPolynomialRingElement = result in
           let i:usize = i in
-          assume (range (v result.(i) * 1441) i32_inttype);
-          let coefficient_normal_form:i32 =
-            Libcrux.Kem.Kyber.Arithmetic.montgomery_reduce ((result
-                    .Libcrux.Kem.Kyber.Arithmetic.f_coefficients.[ i ]
-                  <:
-                  i32) *!
-                1441l
-                <:
-                i32)
+          assume (range (v #i32_inttype result.Libcrux.Kem.Kyber.Arithmetic.f_coefficients.[i] * 1441) i32_inttype);
+          let coefficient_normal_form =
+            Libcrux.Kem.Kyber.Arithmetic.montgomery_reduce 
+                    (Libcrux.Kem.Kyber.Arithmetic.mul_i32_b #3328 #1441
+                    (result.Libcrux.Kem.Kyber.Arithmetic.f_coefficients.[ i ])
+                    (1441l <: Libcrux.Kem.Kyber.Arithmetic.i32_b 1441))
           in
           assume (range (v coefficient_normal_form +
                         v #i32_inttype error_2_.f_coefficients.[ i ]) i32_inttype);
           assume (range (v coefficient_normal_form +
                         v #i32_inttype error_2_.f_coefficients.[ i ] +
                         v #i32_inttype message.f_coefficients.[ i ]) i32_inttype);
-          assume (Libcrux.Kem.Kyber.Arithmetic.barrett_pre (coefficient_normal_form +! error_2_.f_coefficients.[ i ] +! message.f_coefficients.[ i ]));
-          let result:Libcrux.Kem.Kyber.Arithmetic.t_PolynomialRingElement =
+//          assume (Libcrux.Kem.Kyber.Arithmetic.barrett_pre (coefficient_normal_form +! error_2_.f_coefficients.[ i ] +! message.f_coefficients.[ i ]));
+          let result:Libcrux.Kem.Kyber.Arithmetic.wfPolynomialRingElement =
             {
               result with
               Libcrux.Kem.Kyber.Arithmetic.f_coefficients
@@ -272,7 +269,7 @@ let compute_ring_element_v
                   i32)
             }
             <:
-            Libcrux.Kem.Kyber.Arithmetic.t_PolynomialRingElement
+            Libcrux.Kem.Kyber.Arithmetic.wfPolynomialRingElement
           in
           result)
   in
@@ -281,59 +278,60 @@ let compute_ring_element_v
 
 let compute_vector_u
       (v_K: usize)
-      (a_as_ntt: t_Array (t_Array Libcrux.Kem.Kyber.Arithmetic.t_PolynomialRingElement v_K) v_K)
-      (r_as_ntt error_1_: t_Array Libcrux.Kem.Kyber.Arithmetic.t_PolynomialRingElement v_K) =
-  let result:t_Array Libcrux.Kem.Kyber.Arithmetic.t_PolynomialRingElement v_K =
+      (a_as_ntt: t_Array (t_Array Libcrux.Kem.Kyber.Arithmetic.wfPolynomialRingElement v_K) v_K)
+      (r_as_ntt error_1_: t_Array Libcrux.Kem.Kyber.Arithmetic.wfPolynomialRingElement v_K) =
+  let result:t_Array Libcrux.Kem.Kyber.Arithmetic.wfPolynomialRingElement v_K =
     Rust_primitives.Hax.repeat Libcrux.Kem.Kyber.Arithmetic.impl__PolynomialRingElement__ZERO v_K
   in
-  let acc_t = t_Array Libcrux.Kem.Kyber.Arithmetic.t_PolynomialRingElement v_K in
+  let acc_t = t_Array Libcrux.Kem.Kyber.Arithmetic.wfPolynomialRingElement v_K in
   [@ inline_let]
   let inv = fun (acc:acc_t) (i:usize) -> True in
-  let result:t_Array Libcrux.Kem.Kyber.Arithmetic.t_PolynomialRingElement v_K =
-    Rust_primitives.Iterators.foldi_slice #(t_Array Libcrux.Kem.Kyber.Arithmetic.t_PolynomialRingElement v_K) #acc_t #inv
+  let result:t_Array Libcrux.Kem.Kyber.Arithmetic.wfPolynomialRingElement v_K =
+    Rust_primitives.Iterators.foldi_slice #(t_Array Libcrux.Kem.Kyber.Arithmetic.wfPolynomialRingElement v_K) #acc_t #inv
       a_as_ntt
       result
       (fun result temp_1_ ->
-          let result:t_Array Libcrux.Kem.Kyber.Arithmetic.t_PolynomialRingElement v_K = result in
-          let i, row:(usize & t_Array Libcrux.Kem.Kyber.Arithmetic.t_PolynomialRingElement v_K) =
+          let result:t_Array Libcrux.Kem.Kyber.Arithmetic.wfPolynomialRingElement v_K = result in
+          let i, row:(usize & t_Array Libcrux.Kem.Kyber.Arithmetic.wfPolynomialRingElement v_K) =
             temp_1_
           in
           [@ inline_let]
           let inv = fun (acc:acc_t) (i:usize) -> True in
-          let result:t_Array Libcrux.Kem.Kyber.Arithmetic.t_PolynomialRingElement v_K =
-            Rust_primitives.Iterators.foldi_slice #Libcrux.Kem.Kyber.Arithmetic.t_PolynomialRingElement #acc_t #inv
+          let result:t_Array Libcrux.Kem.Kyber.Arithmetic.wfPolynomialRingElement v_K =
+            Rust_primitives.Iterators.foldi_slice #Libcrux.Kem.Kyber.Arithmetic.wfPolynomialRingElement #acc_t #inv
               row
               result
               (fun result temp_1_ ->
-                  let result:t_Array Libcrux.Kem.Kyber.Arithmetic.t_PolynomialRingElement v_K =
+                  let result:t_Array Libcrux.Kem.Kyber.Arithmetic.wfPolynomialRingElement v_K =
                     result
                   in
-                  let j, a_element:(usize & Libcrux.Kem.Kyber.Arithmetic.t_PolynomialRingElement) =
+                  let j, a_element:(usize & Libcrux.Kem.Kyber.Arithmetic.wfPolynomialRingElement) =
                     temp_1_
                   in
-                  let product:Libcrux.Kem.Kyber.Arithmetic.t_PolynomialRingElement =
+                  admit();
+                  let product:Libcrux.Kem.Kyber.Arithmetic.wfPolynomialRingElement =
                     Libcrux.Kem.Kyber.Ntt.ntt_multiply a_element
-                      (r_as_ntt.[ j ] <: Libcrux.Kem.Kyber.Arithmetic.t_PolynomialRingElement)
+                      (r_as_ntt.[ j ] <: Libcrux.Kem.Kyber.Arithmetic.wfPolynomialRingElement)
                   in
                   admit(); //pre for add_to_ring
-                  let result:t_Array Libcrux.Kem.Kyber.Arithmetic.t_PolynomialRingElement v_K =
+                  let result:t_Array Libcrux.Kem.Kyber.Arithmetic.wfPolynomialRingElement v_K =
                     Rust_primitives.Hax.Monomorphized_update_at.update_at_usize result
                       i
                       (Libcrux.Kem.Kyber.Arithmetic.add_to_ring_element v_K
-                          (result.[ i ] <: Libcrux.Kem.Kyber.Arithmetic.t_PolynomialRingElement)
+                          (result.[ i ] <: Libcrux.Kem.Kyber.Arithmetic.wfPolynomialRingElement)
                           product
                         <:
-                        Libcrux.Kem.Kyber.Arithmetic.t_PolynomialRingElement)
+                        Libcrux.Kem.Kyber.Arithmetic.wfPolynomialRingElement)
                   in
                   result)
           in
-          let result:t_Array Libcrux.Kem.Kyber.Arithmetic.t_PolynomialRingElement v_K =
+          let result:t_Array Libcrux.Kem.Kyber.Arithmetic.wfPolynomialRingElement v_K =
             Rust_primitives.Hax.Monomorphized_update_at.update_at_usize result
               i
               (Libcrux.Kem.Kyber.Ntt.invert_ntt_montgomery v_K
-                  (result.[ i ] <: Libcrux.Kem.Kyber.Arithmetic.t_PolynomialRingElement)
+                  (result.[ i ] <: Libcrux.Kem.Kyber.Arithmetic.wfPolynomialRingElement)
                 <:
-                Libcrux.Kem.Kyber.Arithmetic.t_PolynomialRingElement)
+                Libcrux.Kem.Kyber.Arithmetic.wfPolynomialRingElement)
           in
           Core.Iter.Traits.Iterator.f_fold (Core.Iter.Traits.Collect.f_into_iter ({
                     Core.Ops.Range.f_start = sz 0;
@@ -347,41 +345,41 @@ let compute_vector_u
               Core.Ops.Range.t_Range usize)
             result
             (fun result j ->
-                let result:t_Array Libcrux.Kem.Kyber.Arithmetic.t_PolynomialRingElement v_K =
+                let result:t_Array Libcrux.Kem.Kyber.Arithmetic.wfPolynomialRingElement v_K =
                   result
                 in
                 assume (range (v (result.[i]).(j) * 1441) i32_inttype);
 
                 let j:usize = j in
-                let coefficient_normal_form:i32 =
-                  Libcrux.Kem.Kyber.Arithmetic.montgomery_reduce (((result.[ i ]
+                let coefficient_normal_form =
+                  Libcrux.Kem.Kyber.Arithmetic.montgomery_reduce (
+                  Libcrux.Kem.Kyber.Arithmetic.mul_i32_b
+                  ((result.[ i ]
                           <:
-                          Libcrux.Kem.Kyber.Arithmetic.t_PolynomialRingElement)
+                          Libcrux.Kem.Kyber.Arithmetic.wfPolynomialRingElement)
                           .Libcrux.Kem.Kyber.Arithmetic.f_coefficients.[ j ]
                         <:
-                        i32) *!
-                      1441l
-                      <:
-                      i32)
+                        Libcrux.Kem.Kyber.Arithmetic.i32_b 3328)
+                   (1441l <: Libcrux.Kem.Kyber.Arithmetic.i32_b 1441)) 
                 in
                 assume (range (v coefficient_normal_form + v (error_1_.[i]).( j )) i32_inttype);
-                assume (Libcrux.Kem.Kyber.Arithmetic.barrett_pre (coefficient_normal_form +! (error_1_.[i]).( j ))); 
-                let result:t_Array Libcrux.Kem.Kyber.Arithmetic.t_PolynomialRingElement v_K =
+//                assume (Libcrux.Kem.Kyber.Arithmetic.barrett_pre (coefficient_normal_form +! (error_1_.[i]).( j ))); 
+                let result:t_Array Libcrux.Kem.Kyber.Arithmetic.wfPolynomialRingElement v_K =
                   Rust_primitives.Hax.Monomorphized_update_at.update_at_usize result
                     i
                     ({
-                        (result.[ i ] <: Libcrux.Kem.Kyber.Arithmetic.t_PolynomialRingElement) with
+                        (result.[ i ] <: Libcrux.Kem.Kyber.Arithmetic.wfPolynomialRingElement) with
                         Libcrux.Kem.Kyber.Arithmetic.f_coefficients
                         =
                         Rust_primitives.Hax.Monomorphized_update_at.update_at_usize (result.[ i ]
                             <:
-                            Libcrux.Kem.Kyber.Arithmetic.t_PolynomialRingElement)
+                            Libcrux.Kem.Kyber.Arithmetic.wfPolynomialRingElement)
                             .Libcrux.Kem.Kyber.Arithmetic.f_coefficients
                           j
                           (Libcrux.Kem.Kyber.Arithmetic.barrett_reduce (coefficient_normal_form +!
                                 ((error_1_.[ i ]
                                     <:
-                                    Libcrux.Kem.Kyber.Arithmetic.t_PolynomialRingElement)
+                                    Libcrux.Kem.Kyber.Arithmetic.wfPolynomialRingElement)
                                     .Libcrux.Kem.Kyber.Arithmetic.f_coefficients.[ j ]
                                   <:
                                   i32)
@@ -393,7 +391,7 @@ let compute_vector_u
                         t_Array i32 (sz 256)
                       }
                       <:
-                      Libcrux.Kem.Kyber.Arithmetic.t_PolynomialRingElement)
+                      Libcrux.Kem.Kyber.Arithmetic.wfPolynomialRingElement)
                 in
                 result))
   in
@@ -401,14 +399,14 @@ let compute_vector_u
   result
 
 let sample_matrix_A (v_K: usize) (seed: t_Array u8 (sz 34)) (transpose: bool) =
-  let v_A_transpose:t_Array (t_Array Libcrux.Kem.Kyber.Arithmetic.t_PolynomialRingElement v_K) v_K =
+  let v_A_transpose:t_Array (t_Array Libcrux.Kem.Kyber.Arithmetic.wfPolynomialRingElement v_K) v_K =
     Rust_primitives.Hax.repeat (Rust_primitives.Hax.repeat Libcrux.Kem.Kyber.Arithmetic.impl__PolynomialRingElement__ZERO
           v_K
         <:
-        t_Array Libcrux.Kem.Kyber.Arithmetic.t_PolynomialRingElement v_K)
+        t_Array Libcrux.Kem.Kyber.Arithmetic.wfPolynomialRingElement v_K)
       v_K
   in
-  let v_A_transpose:t_Array (t_Array Libcrux.Kem.Kyber.Arithmetic.t_PolynomialRingElement v_K) v_K =
+  let v_A_transpose:t_Array (t_Array Libcrux.Kem.Kyber.Arithmetic.wfPolynomialRingElement v_K) v_K =
     Core.Iter.Traits.Iterator.f_fold (Core.Iter.Traits.Collect.f_into_iter ({
               Core.Ops.Range.f_start = sz 0;
               Core.Ops.Range.f_end = v_K
@@ -420,7 +418,7 @@ let sample_matrix_A (v_K: usize) (seed: t_Array u8 (sz 34)) (transpose: bool) =
       v_A_transpose
       (fun v_A_transpose i ->
           let v_A_transpose:t_Array
-            (t_Array Libcrux.Kem.Kyber.Arithmetic.t_PolynomialRingElement v_K) v_K =
+            (t_Array Libcrux.Kem.Kyber.Arithmetic.wfPolynomialRingElement v_K) v_K =
             v_A_transpose
           in
           let i:usize = i in
@@ -476,11 +474,11 @@ let sample_matrix_A (v_K: usize) (seed: t_Array u8 (sz 34)) (transpose: bool) =
             v_A_transpose
             (fun v_A_transpose j ->
                 let v_A_transpose:t_Array
-                  (t_Array Libcrux.Kem.Kyber.Arithmetic.t_PolynomialRingElement v_K) v_K =
+                  (t_Array Libcrux.Kem.Kyber.Arithmetic.wfPolynomialRingElement v_K) v_K =
                   v_A_transpose
                 in
                 let j:usize = j in
-                let sampled:Libcrux.Kem.Kyber.Arithmetic.t_PolynomialRingElement =
+                let sampled:Libcrux.Kem.Kyber.Arithmetic.wfPolynomialRingElement =
                   Libcrux.Kem.Kyber.Sampling.sample_from_uniform_distribution (xof_bytes.[ j ]
                       <:
                       t_Array u8 (sz 840))
@@ -488,32 +486,32 @@ let sample_matrix_A (v_K: usize) (seed: t_Array u8 (sz 34)) (transpose: bool) =
                 if transpose
                 then
                   let v_A_transpose:t_Array
-                    (t_Array Libcrux.Kem.Kyber.Arithmetic.t_PolynomialRingElement v_K) v_K =
+                    (t_Array Libcrux.Kem.Kyber.Arithmetic.wfPolynomialRingElement v_K) v_K =
                     Rust_primitives.Hax.Monomorphized_update_at.update_at_usize v_A_transpose
                       j
                       (Rust_primitives.Hax.Monomorphized_update_at.update_at_usize (v_A_transpose.[ j
                             ]
                             <:
-                            t_Array Libcrux.Kem.Kyber.Arithmetic.t_PolynomialRingElement v_K)
+                            t_Array Libcrux.Kem.Kyber.Arithmetic.wfPolynomialRingElement v_K)
                           i
                           sampled
                         <:
-                        t_Array Libcrux.Kem.Kyber.Arithmetic.t_PolynomialRingElement v_K)
+                        t_Array Libcrux.Kem.Kyber.Arithmetic.wfPolynomialRingElement v_K)
                   in
                   v_A_transpose
                 else
                   let v_A_transpose:t_Array
-                    (t_Array Libcrux.Kem.Kyber.Arithmetic.t_PolynomialRingElement v_K) v_K =
+                    (t_Array Libcrux.Kem.Kyber.Arithmetic.wfPolynomialRingElement v_K) v_K =
                     Rust_primitives.Hax.Monomorphized_update_at.update_at_usize v_A_transpose
                       i
                       (Rust_primitives.Hax.Monomorphized_update_at.update_at_usize (v_A_transpose.[ i
                             ]
                             <:
-                            t_Array Libcrux.Kem.Kyber.Arithmetic.t_PolynomialRingElement v_K)
+                            t_Array Libcrux.Kem.Kyber.Arithmetic.wfPolynomialRingElement v_K)
                           j
                           sampled
                         <:
-                        t_Array Libcrux.Kem.Kyber.Arithmetic.t_PolynomialRingElement v_K)
+                        t_Array Libcrux.Kem.Kyber.Arithmetic.wfPolynomialRingElement v_K)
                   in
                   v_A_transpose))
   in
