proofs/fstar/extraction-edited/Libcrux.Kem.Kyber.Matrix.fsti
@@ -3,68 +3,69 @@ module Libcrux.Kem.Kyber.Matrix
 open Core
 open FStar.Mul
 
+
 val compute_As_plus_e (#p:Spec.Kyber.params)
       (v_K: usize)
-      (matrix_A: t_Array (t_Array Libcrux.Kem.Kyber.Arithmetic.t_PolynomialRingElement v_K) v_K)
-      (s_as_ntt error_as_ntt: t_Array Libcrux.Kem.Kyber.Arithmetic.t_PolynomialRingElement v_K)
-    : Pure (t_Array Libcrux.Kem.Kyber.Arithmetic.t_PolynomialRingElement v_K) 
+      (matrix_A: t_Array (t_Array Libcrux.Kem.Kyber.Arithmetic.wfPolynomialRingElement v_K) v_K)
+      (s_as_ntt error_as_ntt: t_Array Libcrux.Kem.Kyber.Arithmetic.wfPolynomialRingElement v_K)
+    : Pure (t_Array Libcrux.Kem.Kyber.Arithmetic.wfPolynomialRingElement v_K) 
            (requires (v_K == p.v_RANK))
            (ensures fun res ->
              let open Libcrux.Kem.Kyber.Arithmetic in
              v_K == p.v_RANK /\
-             to_spec_vector #p res =
+             to_spec_vector_b #p res =
              Spec.Kyber.compute_As_plus_e #p
-               (to_spec_matrix #p matrix_A) 
-               (to_spec_vector #p s_as_ntt) 
-               (to_spec_vector #p error_as_ntt))
+               (to_spec_matrix_b #p matrix_A) 
+               (to_spec_vector_b #p s_as_ntt) 
+               (to_spec_vector_b #p error_as_ntt))
 
 
 val compute_message (#p:Spec.Kyber.params)
       (v_K: usize)
-      (poly_v: Libcrux.Kem.Kyber.Arithmetic.t_PolynomialRingElement)
-      (secret_as_ntt u_as_ntt: t_Array Libcrux.Kem.Kyber.Arithmetic.t_PolynomialRingElement v_K)
-    : Pure (Libcrux.Kem.Kyber.Arithmetic.t_PolynomialRingElement)
+      (poly_v: Libcrux.Kem.Kyber.Arithmetic.wfPolynomialRingElement)
+      (secret_as_ntt u_as_ntt: t_Array Libcrux.Kem.Kyber.Arithmetic.wfPolynomialRingElement v_K)
+    : Pure (Libcrux.Kem.Kyber.Arithmetic.wfPolynomialRingElement)
       (requires (v_K == p.v_RANK))
       (ensures (fun res -> 
-        let secret_spec = Libcrux.Kem.Kyber.Arithmetic.to_spec_vector #p secret_as_ntt in
-        let u_spec = Libcrux.Kem.Kyber.Arithmetic.to_spec_vector #p u_as_ntt in
-        let v_spec = Libcrux.Kem.Kyber.Arithmetic.to_spec_poly poly_v in
-        Libcrux.Kem.Kyber.Arithmetic.to_spec_poly res ==
+        let secret_spec = Libcrux.Kem.Kyber.Arithmetic.to_spec_vector_b #p secret_as_ntt in
+        let u_spec = Libcrux.Kem.Kyber.Arithmetic.to_spec_vector_b #p u_as_ntt in
+        let v_spec = Libcrux.Kem.Kyber.Arithmetic.to_spec_poly_b poly_v in
+        Libcrux.Kem.Kyber.Arithmetic.to_spec_poly_b res ==
         Spec.Kyber.(poly_sub v_spec (poly_inv_ntt #p (vector_dot_product secret_spec u_spec)))))
 
 val compute_ring_element_v (#p:Spec.Kyber.params)
       (v_K: usize)
-      (tt_as_ntt r_as_ntt: t_Array Libcrux.Kem.Kyber.Arithmetic.t_PolynomialRingElement v_K)
-      (error_2_ message: Libcrux.Kem.Kyber.Arithmetic.t_PolynomialRingElement)
-    : Pure (Libcrux.Kem.Kyber.Arithmetic.t_PolynomialRingElement)
+      (tt_as_ntt r_as_ntt: t_Array Libcrux.Kem.Kyber.Arithmetic.wfPolynomialRingElement v_K)
+      (error_2_ message: Libcrux.Kem.Kyber.Arithmetic.wfPolynomialRingElement)
+    : Pure (Libcrux.Kem.Kyber.Arithmetic.wfPolynomialRingElement)
       (requires (v_K == p.v_RANK))
       (ensures fun res ->
-        let tt_spec = Libcrux.Kem.Kyber.Arithmetic.to_spec_vector #p tt_as_ntt in
-        let r_spec = Libcrux.Kem.Kyber.Arithmetic.to_spec_vector #p r_as_ntt in
-        let e2_spec = Libcrux.Kem.Kyber.Arithmetic.to_spec_poly error_2_ in
-        let m_spec = Libcrux.Kem.Kyber.Arithmetic.to_spec_poly message in
-        let res_spec = Libcrux.Kem.Kyber.Arithmetic.to_spec_poly res in
+        let tt_spec = Libcrux.Kem.Kyber.Arithmetic.to_spec_vector_b #p tt_as_ntt in
+        let r_spec = Libcrux.Kem.Kyber.Arithmetic.to_spec_vector_b #p r_as_ntt in
+        let e2_spec = Libcrux.Kem.Kyber.Arithmetic.to_spec_poly_b error_2_ in
+        let m_spec = Libcrux.Kem.Kyber.Arithmetic.to_spec_poly_b message in
+        let res_spec = Libcrux.Kem.Kyber.Arithmetic.to_spec_poly_b res in
         res_spec == Spec.Kyber.(poly_add (poly_add (vector_dot_product tt_spec r_spec) e2_spec) m_spec))
 
 val compute_vector_u (#p:Spec.Kyber.params)
       (v_K: usize)
-      (a_as_ntt: t_Array (t_Array Libcrux.Kem.Kyber.Arithmetic.t_PolynomialRingElement v_K) v_K)
-      (r_as_ntt error_1_: t_Array Libcrux.Kem.Kyber.Arithmetic.t_PolynomialRingElement v_K)
-    : Pure (t_Array Libcrux.Kem.Kyber.Arithmetic.t_PolynomialRingElement v_K)
+      (a_as_ntt: t_Array (t_Array Libcrux.Kem.Kyber.Arithmetic.wfPolynomialRingElement v_K) v_K)
+      (r_as_ntt error_1_: t_Array Libcrux.Kem.Kyber.Arithmetic.wfPolynomialRingElement v_K)
+    : Pure (t_Array Libcrux.Kem.Kyber.Arithmetic.wfPolynomialRingElement v_K)
       (requires (v_K == p.v_RANK))
       (ensures fun res ->
-        let a_spec = Libcrux.Kem.Kyber.Arithmetic.to_spec_matrix #p a_as_ntt in
-        let r_spec = Libcrux.Kem.Kyber.Arithmetic.to_spec_vector #p r_as_ntt in
-        let e_spec = Libcrux.Kem.Kyber.Arithmetic.to_spec_vector #p error_1_ in
-        let res_spec = Libcrux.Kem.Kyber.Arithmetic.to_spec_vector #p res in
+        let a_spec = Libcrux.Kem.Kyber.Arithmetic.to_spec_matrix_b #p a_as_ntt in
+        let r_spec = Libcrux.Kem.Kyber.Arithmetic.to_spec_vector_b #p r_as_ntt in
+        let e_spec = Libcrux.Kem.Kyber.Arithmetic.to_spec_vector_b #p error_1_ in
+        let res_spec = Libcrux.Kem.Kyber.Arithmetic.to_spec_vector_b #p res in
         res_spec == Spec.Kyber.(vector_add (vector_inv_ntt (matrix_vector_mul a_spec r_spec)) e_spec))
 
 
 
 val sample_matrix_A (#p:Spec.Kyber.params) (v_K: usize) (seed: t_Array u8 (sz 34)) (transpose: bool)
-    : Pure (t_Array (t_Array Libcrux.Kem.Kyber.Arithmetic.t_PolynomialRingElement v_K) v_K)
+    : Pure (t_Array (t_Array Libcrux.Kem.Kyber.Arithmetic.wfPolynomialRingElement v_K) v_K)
       (requires (v_K == p.v_RANK))
       (ensures fun res ->
         let matrix_A = Spec.Kyber.sample_matrix_A #p (Seq.slice seed 0 32) in
-        if transpose then Libcrux.Kem.Kyber.Arithmetic.to_spec_matrix #p res == matrix_A
-        else Libcrux.Kem.Kyber.Arithmetic.to_spec_matrix #p res == Spec.Kyber.matrix_transpose matrix_A)
+        if transpose then Libcrux.Kem.Kyber.Arithmetic.to_spec_matrix_b #p res == matrix_A
+        else Libcrux.Kem.Kyber.Arithmetic.to_spec_matrix_b #p res == Spec.Kyber.matrix_transpose matrix_A)
