proofs/fstar/extraction-edited/Libcrux.Kem.Kyber.Sampling.fsti
@@ -4,24 +4,24 @@ open Core
 open FStar.Mul
 
 val sample_from_binomial_distribution_2_ (randomness: t_Slice u8)
-    : Prims.Pure Libcrux.Kem.Kyber.Arithmetic.t_PolynomialRingElement
+    : Prims.Pure Libcrux.Kem.Kyber.Arithmetic.wfPolynomialRingElement
       (requires (Core.Slice.impl__len randomness <: usize) =. (sz 2 *! sz 64 <: usize))
       (ensures
         fun result ->
-          let result:Libcrux.Kem.Kyber.Arithmetic.t_PolynomialRingElement = result in
-          Libcrux.Kem.Kyber.Arithmetic.to_spec_poly result == 
+          let result:Libcrux.Kem.Kyber.Arithmetic.wfPolynomialRingElement = result in
+          Libcrux.Kem.Kyber.Arithmetic.to_spec_poly_b result == 
           Spec.Kyber.sample_poly_binomial (sz 2) randomness /\
           (forall (i:usize). i <. length result.Libcrux.Kem.Kyber.Arithmetic.f_coefficients ==>
              (v #i32_inttype result.f_coefficients.[i] >= - 2 /\
               v #i32_inttype result.f_coefficients.[i] <= 2)))
 
 val sample_from_binomial_distribution_3_ (randomness: t_Slice u8)
-    : Prims.Pure Libcrux.Kem.Kyber.Arithmetic.t_PolynomialRingElement
+    : Prims.Pure Libcrux.Kem.Kyber.Arithmetic.wfPolynomialRingElement
       (requires (Core.Slice.impl__len randomness <: usize) =. (sz 3 *! sz 64 <: usize))
       (ensures
         fun result ->
-          let result:Libcrux.Kem.Kyber.Arithmetic.t_PolynomialRingElement = result in
-          Libcrux.Kem.Kyber.Arithmetic.to_spec_poly result == 
+          let result:Libcrux.Kem.Kyber.Arithmetic.wfPolynomialRingElement = result in
+          Libcrux.Kem.Kyber.Arithmetic.to_spec_poly_b result == 
           Spec.Kyber.sample_poly_binomial (sz 3) randomness /\
          (forall (i:usize). i <. length result.Libcrux.Kem.Kyber.Arithmetic.f_coefficients ==>
              (v #i32_inttype result.f_coefficients.[i] >= -3 /\
@@ -29,13 +29,13 @@ val sample_from_binomial_distribution_3_ (randomness: t_Slice u8)
 
 val sample_from_binomial_distribution (#p:Spec.Kyber.params)
     (v_ETA: usize) (randomness: t_Slice u8)
-    : Pure Libcrux.Kem.Kyber.Arithmetic.t_PolynomialRingElement
+    : Pure Libcrux.Kem.Kyber.Arithmetic.wfPolynomialRingElement
       (requires (v_ETA = p.v_ETA1 \/ v_ETA = p.v_ETA2) /\
                 (Core.Slice.impl__len randomness <: usize) =. (v_ETA *! sz 64 <: usize))
       (ensures
         fun result ->
-          let result:Libcrux.Kem.Kyber.Arithmetic.t_PolynomialRingElement = result in
-          Libcrux.Kem.Kyber.Arithmetic.to_spec_poly result == 
+          let result:Libcrux.Kem.Kyber.Arithmetic.wfPolynomialRingElement = result in
+          Libcrux.Kem.Kyber.Arithmetic.to_spec_poly_b result == 
           Spec.Kyber.sample_poly_binomial v_ETA randomness /\
           (forall (i:usize). i <. length result.Libcrux.Kem.Kyber.Arithmetic.f_coefficients ==>
              (v #i32_inttype result.f_coefficients.[i] >= - (v v_ETA) /\
@@ -43,4 +43,4 @@ val sample_from_binomial_distribution (#p:Spec.Kyber.params)
 
 
 val sample_from_uniform_distribution (randomness: t_Array u8 (sz 840))
-    : Libcrux.Kem.Kyber.Arithmetic.t_PolynomialRingElement 
+    : Libcrux.Kem.Kyber.Arithmetic.wfPolynomialRingElement 
