proofs/fstar/extraction-edited/Libcrux.Kem.Kyber.Serialize.PartB.fsti
@@ -4,45 +4,35 @@ open Core
 open FStar.Mul
 open MkSeq
 
-let is_fe fe = 
-  fe >= v (Core.Ops.Arith.Neg.neg Libcrux.Kem.Kyber.Constants.v_FIELD_MODULUS <: i32) &&
-  fe < v Libcrux.Kem.Kyber.Constants.v_FIELD_MODULUS
-  
-let is_polynomialRingElement_wf re =
-  forall i. i < 256 ==> is_fe (v (re.Libcrux.Kem.Kyber.Arithmetic.f_coefficients.[sz i] <: i32))
-
-type wfPolynomialRingElement =
-  re: Libcrux.Kem.Kyber.Arithmetic.t_PolynomialRingElement {is_polynomialRingElement_wf re}
-
 val compress_then_serialize_10_
       (v_OUT_LEN: usize)
-      (re: wfPolynomialRingElement)
+      (re: Libcrux.Kem.Kyber.Arithmetic.wfPolynomialRingElement)
     : Prims.Pure (t_Array u8 v_OUT_LEN) Prims.l_True (fun _ -> Prims.l_True)
 
 val compress_then_serialize_11_
       (v_OUT_LEN: usize)
-      (re: wfPolynomialRingElement)
+      (re: Libcrux.Kem.Kyber.Arithmetic.wfPolynomialRingElement)
     : Prims.Pure (t_Array u8 v_OUT_LEN) Prims.l_True (fun _ -> Prims.l_True)
 
 val compress_then_serialize_4_
       (v_OUT_LEN: usize)
-      (re: wfPolynomialRingElement)
+      (re: Libcrux.Kem.Kyber.Arithmetic.wfPolynomialRingElement)
     : Prims.Pure (t_Array u8 v_OUT_LEN) Prims.l_True (fun _ -> Prims.l_True)
 
 val compress_then_serialize_5_
       (v_OUT_LEN: usize)
-      (re: wfPolynomialRingElement)
+      (re: Libcrux.Kem.Kyber.Arithmetic.wfPolynomialRingElement)
     : Prims.Pure (t_Array u8 v_OUT_LEN) Prims.l_True (fun _ -> Prims.l_True)
 
-val compress_then_serialize_message (re: wfPolynomialRingElement)
+val compress_then_serialize_message (re: Libcrux.Kem.Kyber.Arithmetic.wfPolynomialRingElement)
     : Pure (t_Array u8 (sz 32))
       (requires True)
       (ensures (fun res ->
-        res == Spec.Kyber.compress_then_encode_message (Libcrux.Kem.Kyber.Arithmetic.to_spec_poly re)))
+        res == Spec.Kyber.compress_then_encode_message (Libcrux.Kem.Kyber.Arithmetic.to_spec_poly_b re)))
 
 val compress_then_serialize_ring_element_u (#p:Spec.Kyber.params)
       (v_COMPRESSION_FACTOR v_OUT_LEN: usize)
-      (re: wfPolynomialRingElement)
+      (re: Libcrux.Kem.Kyber.Arithmetic.wfPolynomialRingElement)
     : Pure (t_Array u8 v_OUT_LEN)
       (requires (v_COMPRESSION_FACTOR = sz 10 || v_COMPRESSION_FACTOR = sz 11) /\
                 v_OUT_LEN = Spec.Kyber.v_C1_BLOCK_SIZE p) 
@@ -50,66 +40,66 @@ val compress_then_serialize_ring_element_u (#p:Spec.Kyber.params)
       
 val compress_then_serialize_ring_element_v (#p:Spec.Kyber.params)
       (v_COMPRESSION_FACTOR v_OUT_LEN: usize)
-      (re: wfPolynomialRingElement)
+      (re: Libcrux.Kem.Kyber.Arithmetic.wfPolynomialRingElement)
     : Pure (t_Array u8 v_OUT_LEN)
       (requires (v_COMPRESSION_FACTOR = sz 4 || v_COMPRESSION_FACTOR = sz 5) /\
                  v_OUT_LEN = Spec.Kyber.v_C2_SIZE p)
       (ensures (fun res -> 
         res == 
         Spec.Kyber.compress_then_encode_v p 
-          (Libcrux.Kem.Kyber.Arithmetic.to_spec_poly re)))
+          (Libcrux.Kem.Kyber.Arithmetic.to_spec_poly_b re)))
 
 val deserialize_then_decompress_10_ (serialized: t_Slice u8)
-    : Prims.Pure Libcrux.Kem.Kyber.Arithmetic.t_PolynomialRingElement
+    : Prims.Pure Libcrux.Kem.Kyber.Arithmetic.wfPolynomialRingElement
       Prims.l_True
       (fun _ -> Prims.l_True)
 
 val deserialize_then_decompress_11_ (serialized: t_Slice u8)
-    : Prims.Pure Libcrux.Kem.Kyber.Arithmetic.t_PolynomialRingElement
+    : Prims.Pure Libcrux.Kem.Kyber.Arithmetic.wfPolynomialRingElement
       Prims.l_True
       (fun _ -> Prims.l_True)
 
 val deserialize_then_decompress_4_ (serialized: t_Slice u8)
-    : Prims.Pure Libcrux.Kem.Kyber.Arithmetic.t_PolynomialRingElement
+    : Prims.Pure Libcrux.Kem.Kyber.Arithmetic.wfPolynomialRingElement
       Prims.l_True
       (fun _ -> Prims.l_True)
 
 val deserialize_then_decompress_5_ (serialized: t_Slice u8)
-    : Prims.Pure Libcrux.Kem.Kyber.Arithmetic.t_PolynomialRingElement
+    : Prims.Pure Libcrux.Kem.Kyber.Arithmetic.wfPolynomialRingElement
       Prims.l_True
       (fun _ -> Prims.l_True)
 
 val deserialize_then_decompress_message (serialized: t_Array u8 (sz 32))
-    : Pure (Libcrux.Kem.Kyber.Arithmetic.t_PolynomialRingElement)
+    : Pure (Libcrux.Kem.Kyber.Arithmetic.wfPolynomialRingElement)
       (requires True)
       (ensures fun res ->
-        Libcrux.Kem.Kyber.Arithmetic.to_spec_poly res == 
+        Libcrux.Kem.Kyber.Arithmetic.to_spec_poly_b res == 
         Spec.Kyber.decode_then_decompress_message serialized)
 
 val deserialize_then_decompress_ring_element_u
       (v_COMPRESSION_FACTOR: usize)
       (serialized: t_Slice u8)
-    : Pure (wfPolynomialRingElement)
+    : Pure (Libcrux.Kem.Kyber.Arithmetic.wfPolynomialRingElement)
       (requires v_COMPRESSION_FACTOR = sz 10 || v_COMPRESSION_FACTOR = sz 11)
       (ensures fun _ -> True)
 
 val deserialize_then_decompress_ring_element_v (#p:Spec.Kyber.params)
       (v_COMPRESSION_FACTOR: usize)
       (serialized: t_Slice u8)
-    : Pure (Libcrux.Kem.Kyber.Arithmetic.t_PolynomialRingElement)
+    : Pure (Libcrux.Kem.Kyber.Arithmetic.wfPolynomialRingElement)
       (requires (p.v_VECTOR_V_COMPRESSION_FACTOR == v_COMPRESSION_FACTOR /\
                  length serialized == Spec.Kyber.v_C2_SIZE p))
       (ensures fun res ->
-       Libcrux.Kem.Kyber.Arithmetic.to_spec_poly res ==
+       Libcrux.Kem.Kyber.Arithmetic.to_spec_poly_b res ==
        Spec.Kyber.decode_then_decompress_v p serialized)
 
 
 val deserialize_to_uncompressed_ring_element (serialized: t_Slice u8)
-    : Pure (Libcrux.Kem.Kyber.Arithmetic.t_PolynomialRingElement)
+    : Pure (Libcrux.Kem.Kyber.Arithmetic.wfPolynomialRingElement)
       (requires (length serialized == Spec.Kyber.v_BYTES_PER_RING_ELEMENT))
       (ensures fun _ -> True)
 
-val serialize_uncompressed_ring_element (re: Libcrux.Kem.Kyber.Arithmetic.t_PolynomialRingElement)
+val serialize_uncompressed_ring_element (re: Libcrux.Kem.Kyber.Arithmetic.wfPolynomialRingElement)
     : Pure (t_Array u8 (sz 384))
       (requires True)
       (ensures (fun res -> True))
